\documentclass{article}

\title{inf-sup \& sup-inf Relations}
\usepackage{dztex}

\begin{document}

\hpart{Intro} Below I present a proof for a well known relationship between $\inf\sup$ and $\sup\inf$.

\hpart{Helper Lemmas}
To begin let's prove a few lemmas which will simplify our proof below
\begin{lemma}\label{lem:1}
  Given $X \subset \mathbb{R}$ bounded below, $y \in \mathbb{R}$ if $x \ge y \forall x \in X$ then
  $$
    \inf_{x \in X} x \ge y
  $$
\end{lemma}
\begin{proof}
  Since $X$ is bounded below we know $\alpha := \inf\limits_{x \in X} x$ is finite. Suppose, for the sake of contradiction, $\alpha < y$. We know $\forall \, \gamma > 0 \exists x \in X$ such that
  $$
    \alpha + \gamma > x
  $$
  since otherwise $\alpha + \gamma$ would be a lower bound of $X$, but $\alpha + \gamma > \alpha$, contradicting the definition of $\alpha$. In particular $y - \alpha > 0 \implies \exists* \, x \in X$ such that
  $$
    y = \alpha + y - \alpha > x \contradiction x \ge y
  $$
\end{proof}
\begin{lemma}\label{lem:2}
  Let $X \subset \mathbb{R}$ be bounded below then
  $$
    - \inf_{x \in X} x = \sup_{x \in X} -x
  $$
\end{lemma}
\begin{proof}
  Since $X$ is bounded below we know $\alpha := \inf\limits_{x \in X}$ and $\beta := \sup\limits_{x \in X} -x$ are finite. We have $\forall x \in X$
  $$
    \alpha \le x \implies - \alpha \ge -x
  $$
  thus $-\alpha$ is an upper bound on $\{ -x \mid x \in X \}$ so that
  \begin{equation}
    -\alpha \ge \beta \label{eq:1}
  \end{equation}
  Additionally $\forall* \, x \in X$
  $$
    -x \le \beta \implies x \ge -\beta
  $$
  thus $-\beta$ is a lower bound of $X$ so that $\alpha \ge -\beta$ or equivalently
  \begin{equation}
    -\alpha \le \beta \label{eq:2}
  \end{equation}
  Combining \eqref{eq:1} \& \eqref{eq:2} gives us our desired equality.
\end{proof}
\begin{lemma}\label{lem:3}
  Given $X \subset \mathbb{R}$ bounded above, $y \in \mathbb{R}$ if $x \le y \forall x \in X$ then
  $$
    \sup_{x \in X} x \le y
  $$
\end{lemma}
\begin{proof}
  By \cref{lem:2,lem:1} we have
  $$
    -\sup_{x \in X} x = \inf\limits_{x \in X} -x \ge -y \implies \sup_{x \in X} x \le y
  $$
\end{proof}

\hpart{Main Results}

\begin{theorem}
  Let $X, Y$ be two non-empty sets, $Z \subset \mathbb{R}$ and $f : X \times Y \to Z$, then
  $$
    \inf_{x \in X} \sup_{y \in Y} f(x, y) \ge \sup_{y \in Y} \inf_{x \in X} f(x, y)
  $$
\end{theorem}
\begin{proof}
  Let $x' \in X, y' \in Y$ (as $X, Y$ are non-empty we know these exist). We have
  $$
    \sup_{y \in Y} f(x', y) \ge f(x', y') \ge \inf_{x \in X} f(x, y')
  $$
  By \cref{lem:1} we have
  $$
    \inf_{x \in X} \sup_{y \in Y} f(x, y) \ge \inf_{x \in X} f(x, y')
  $$
  and by \cref{lem:3} we have
  $$
    \inf_{x \in X} \sup_{y \in Y} f(x, y) \ge \sup_{y \in Y} \inf{x \in X} f(x, y)
  $$
\end{proof}
\end{document}
